Strata/DDM/Elab.lean
@@ -46,8 +46,8 @@ def initDeclState : DeclState :=
 end DeclState
 
 inductive Header where
-| dialect (stx : Syntax) (name : DialectName)
-| program (stx : Syntax) (name : DialectName)
+| dialect (loc : SourceLoc) (name : DialectName)
+| program (loc : SourceLoc) (name : DialectName)
 deriving Inhabited
 
 /- Elaborate a Strata program -/
@@ -56,7 +56,7 @@ partial def elabHeader
     (inputContext : InputContext)
     (startPos : String.Pos := 0)
     (stopPos : String.Pos := inputContext.input.endPos)
-     : Header × Array (Syntax × Message) × String.Pos :=
+     : Header × Array Message × String.Pos :=
   let s : DeclState := .initDeclState
   let s := s.openLoadedDialect! .builtin headerDialect
   let s := { s with pos := startPos }
@@ -71,8 +71,8 @@ partial def elabHeader
       let name := tree[0]!.info.asIdent!
       let header :=
         match cmd.op.name.name with
-        | "dialectCommand" => .dialect cmd.stx name.val
-        | "programCommand" => .program cmd.stx name.val
+        | "dialectCommand" => .dialect cmd.loc name.val
+        | "programCommand" => .program cmd.loc name.val
         | _ => panic! s!"Unknown command {cmd.op.name}"
       (header, #[], s.pos)
   else
@@ -93,14 +93,13 @@ partial def runCommand (leanEnv : Lean.Environment) (commands : Array Operation)
 
 def elabProgramRest (loader : LoadedDialects) (leanEnv : Lean.Environment)
     (inputContext : InputContext)
-    (stx : Lean.Syntax)
+    (loc : SourceLoc)
     (dialect : DialectName)
     (startPos : String.Pos)
     (stopPos : String.Pos := inputContext.input.endPos)
-    : Except (Array (Syntax × Message)) Program := do
+    : Except (Array Message) Program := do
   let some d := loader.dialects[dialect]?
-    | let pos := stx.getPos? |>.getD 0
-      .error #[(stx, Lean.mkStringMessage inputContext pos s!"Unknown dialect {dialect}.")]
+    | .error #[Lean.mkStringMessage inputContext ⟨loc.start⟩ s!"Unknown dialect {dialect}."]
   let s := DeclState.initDeclState
   let s := { s with pos := startPos }
   let s := s.openLoadedDialect! loader d
@@ -118,18 +117,17 @@ partial def elabProgram
     (leanEnv : Lean.Environment)
     (inputContext : InputContext)
     (startPos : String.Pos := 0)
-    (stopPos : String.Pos := inputContext.input.endPos) : Except (Array (Syntax × Message)) Program :=
+    (stopPos : String.Pos := inputContext.input.endPos) : Except (Array Message) Program :=
   assert! "Init" ∈ loader.dialects
   let (header, errors, startPos) := elabHeader leanEnv inputContext startPos stopPos
   if errors.size > 0 then
     .error errors
   else
     match header with
-    | .dialect stx _ =>
-      let pos := stx.getPos? |>.getD 0
-      .error #[(stx, Lean.mkStringMessage inputContext pos "Expected program name")]
-    | .program stx dialect => do
-      elabProgramRest loader leanEnv inputContext stx dialect startPos stopPos
+    | .dialect loc _ =>
+      .error #[Lean.mkStringMessage inputContext ⟨loc.start⟩ "Expected program name"]
+    | .program loc dialect => do
+      elabProgramRest loader leanEnv inputContext loc dialect startPos stopPos
 
 /--
 Elaborate a dialect after the initial header with the name of dialect
@@ -140,7 +138,7 @@ partial def elabDialectRest
       (loadCallback : LoadDialectCallback)
       (dialects : LoadedDialects)
       (inputContext : Parser.InputContext)
-      (stx : Syntax)
+      (loc : SourceLoc)
       (dialect : DialectName)
       (startPos : String.Pos := 0)
       (stopPos : String.Pos := inputContext.input.endPos)
@@ -161,7 +159,7 @@ partial def elabDialectRest
   }
   let act : DialectM Unit := do
         if dialect ∈ (← get).loaded.dialects then
-          logError stx[1] s!"Dialect {dialect} already declared."
+          logError loc s!"Dialect {dialect} already declared."
         else
           run
   let dctx : DialectContext := {
@@ -193,13 +191,12 @@ def elabDialect
   if errors.size > 0 then
     return (default, { errors := errors }, dialects)
   match header with
-  | .program stx _ =>
-    let pos := stx.getPos? |>.getD 0
+  | .program loc _ =>
     return (default, {
-      errors := #[(stx, Lean.mkStringMessage inputContext pos "Expected dialect name")]
+      errors := #[Lean.mkStringMessage inputContext ⟨loc.start⟩ "Expected dialect name"]
     },
     dialects)
-  | .dialect stx dialect =>
-    elabDialectRest leanEnv loadCallback dialects inputContext stx dialect startPos stopPos
+  | .dialect loc dialect =>
+    elabDialectRest leanEnv loadCallback dialects inputContext loc dialect startPos stopPos
 
 end Strata.Elab
