Strata/DDM/Elab/Core.lean
@@ -16,6 +16,22 @@ open Strata.Parser (DeclParser InputContext ParserState)
 
 namespace Strata
 
+namespace TypeExprF
+
+/-
+This applies global context to instantiate types and variables.
+
+Free type alias variables bound to alias
+-/
+protected def instType (d : TypeExprF α) (bindings : Array (TypeExprF α)) : TypeExprF α := Id.run <|
+  d.instTypeM fun n idx =>
+    if p : idx < bindings.size then
+      pure <| bindings[bindings.size - (idx+1)]
+    else
+      .bvar n (idx - bindings.size)
+
+end TypeExprF
+
 /--
 Get the kind as a qualified identifier.
 -/
@@ -25,22 +41,24 @@ def qualIdentKind (stx : Syntax) : Option QualifiedIdent :=
   else
     none
 
-partial def expandMacros (m : DialectMap) (f : PreType) (args : Nat → Option Arg) : Except Unit TypeExpr :=
+partial def expandMacros (dm : DialectMap) (f : PreType) (args : Nat → Option Arg) : Except Unit TypeExpr :=
   match f with
-  | .ident i a => .ident i <$> a.mapM fun e => expandMacros m e args
-  | .arrow a b => .arrow <$> expandMacros m a args <*> expandMacros m b args
-  | .fvar i a => .fvar i <$> a.mapM fun e => expandMacros m e args
-  | .bvar idx => pure (.bvar idx)
-  | .funMacro i r => do
-    let r ← expandMacros m r args
+  | .ident loc i a => .ident loc i <$> a.mapM fun e => expandMacros dm e args
+  | .arrow loc a b => .arrow loc <$> expandMacros dm a args <*> expandMacros dm b args
+  | .fvar loc i a => .fvar loc i <$> a.mapM fun e => expandMacros dm e args
+  | .bvar loc idx => pure (.bvar loc idx)
+  | .funMacro loc i r => do
+    let r ← expandMacros dm r args
     match args i with
     | none =>
       .error ()
     | some a =>
-      let addType tps _ s args := tps.push (resolveBindingType m s args)
-      let argTypes := foldArgBindingSpecs m addType (init := #[]) a
-      --let argTypes := foldOverArgAtLevel m addType (init := #[]) bindings args level
-      pure <| argTypes.foldr (init := r) .arrow
+      let addType (tps : Array TypeExpr) loc _ s args : Array TypeExpr :=
+        match resolveBindingIndices dm loc s args with
+        | .expr tp => tps.push tp
+        | .type _ _ => panic! s!"Expected binding to be expression."
+      let argTypes := foldOverArgBindingSpecs dm addType (init := #[]) a
+      pure <| argTypes.foldr (init := r) (.arrow loc)
 
 namespace Elab
 
@@ -69,7 +87,7 @@ structure ElabContext where
 
 structure ElabState where
   -- Errors found in elaboration.
-  errors : Array (Syntax × Message) := #[]
+  errors : Array Message := #[]
 
 @[reducible]
 def ElabM α := ReaderT ElabContext (StateM ElabState) α
@@ -80,8 +98,8 @@ instance : ElabClass ElabM where
   getOpenDialects := return (←read).openDialectSet
   getGlobalContext := return (←read).globalContext
   getErrorCount := return (←get).errors.size
-  logErrorMessage stx msg :=
-    modify fun s => { s with errors := s.errors.push (stx, msg) }
+  logErrorMessage msg :=
+    modify fun s => { s with errors := s.errors.push msg }
 
 section
 
@@ -92,23 +110,23 @@ inductive MaybeQualifiedIdent where
 | name : String → MaybeQualifiedIdent
 deriving Inhabited
 
-def resolveTypeBinding (tctx : TypingContext) (stx : Syntax) (name : String)
+def resolveTypeBinding (tctx : TypingContext) (loc : SourceLoc) (name : String)
     (binding : TypingContext.VarBinding) (args : Array Tree) : ElabM Tree := do
   match binding with
   | .bvar idx k =>
     if let some a := args[0]? then
-      logErrorMF a.info.stx mf!"Unexpected arguments to {name}."
+      logErrorMF a.info.loc mf!"Unexpected arguments to {name}."
       return default
     if let .type [] _ := k then
-      let info : TypeInfo := { inputCtx := tctx, stx := stx, typeExpr := .bvar idx, isInferred := false }
+      let info : TypeInfo := { inputCtx := tctx, loc := loc, typeExpr := .bvar loc idx, isInferred := false }
       return .node (.ofTypeInfo info) #[]
     else
-      logErrorMF stx mf!"Expected a type instead of {k}"
+      logErrorMF loc mf!"Expected a type instead of {k}"
       return default
   | .fvar fidx k =>
     match k with
     | .expr tp =>
-      logErrorMF stx mf!"Expected a type instead of expression with type {tp}."
+      logErrorMF loc mf!"Expected a type instead of expression with type {tp}."
       return default
     | .type params _ =>
       let params := params.toArray
@@ -119,31 +137,31 @@ def resolveTypeBinding (tctx : TypingContext) (stx : Syntax) (name : String)
         for i in Fin.range args.size do
           let c := args[i]
           let .ofTypeInfo cinfo := c.info
-            | logErrorMF c.info.stx mf!"Expected type"
+            | logErrorMF c.info.loc mf!"Expected type"
           tpArgs := tpArgs.push cinfo.typeExpr
           children := children.push c
-        let tp :=  .fvar fidx tpArgs
-        let info : TypeInfo := { inputCtx := tctx, stx := stx, typeExpr := tp, isInferred := false }
+        let tp :=  .fvar loc fidx tpArgs
+        let info : TypeInfo := { inputCtx := tctx, loc := loc, typeExpr := tp, isInferred := false }
         return .node (.ofTypeInfo info) children
       else if let some a := args[params.size]? then
-        logErrorMF a.info.stx mf!"Unexpected argument to {name}."
+        logErrorMF a.info.loc mf!"Unexpected argument to {name}."
         return default
       else
-        logErrorMF stx mf!"{name} expects {params.size} arguments."
+        logErrorMF loc mf!"{name} expects {params.size} arguments."
         return default
 
 /--
 This translate a possibly qualified identifier into a declaration in an
 open dialect.
 -/
-def resolveTypeOrCat (stx : Syntax) (tpId : MaybeQualifiedIdent) : ElabM (Option (QualifiedIdent × TypeOrCatDecl)) :=
+def resolveTypeOrCat (loc : SourceLoc) (tpId : MaybeQualifiedIdent) : ElabM (Option (QualifiedIdent × TypeOrCatDecl)) := do
   match tpId with
   | .qid qid => do
     let decls := (← read).typeOrCatDeclMap.get qid.name
     let decls := decls.filter fun (dialect, _) => dialect = qid.dialect
     match decls[0]? with
     | none => do
-      logErrorMF stx mf!"Undeclared type or category {qid}."
+      logErrorMF loc mf!"Undeclared type or category {qid}."
       return none
     | some (_, decl) =>
       assert! decls.size = 1
@@ -153,12 +171,12 @@ def resolveTypeOrCat (stx : Syntax) (tpId : MaybeQualifiedIdent) : ElabM (Option
     let decls:= m.get name
     match decls[0]? with
     | none => do
-      logErrorMF stx mf!"Undeclared type or category {name}."
+      logErrorMF loc mf!"Undeclared type or category {name}."
       return none
     | some (d, decl) =>
       if let some (candD, _) := decls[1]? then
         assert! d ≠ candD
-        logError stx s!"{name} is ambiguous: declared in {d} and {candD}."
+        logError loc s!"{name} is ambiguous: declared in {d} and {candD}."
         return none
       else
         return some ({ dialect := d, name }, decl.val)
@@ -180,40 +198,40 @@ def asTypeInfo (tree : Tree) : ElabM TypeInfo := do
   | .ofTypeInfo info =>
     return info
   | _ =>
-    logError tree.info.stx "Expected type."
+    logError tree.info.loc "Expected type."
     return default
 
-def checkArgSize {α} [ToStrataFormat α] (stx : Syntax) (name : α) (expected : Nat) (args : Array Tree) : ElabM Unit := do
+def checkArgSize {α} [ToStrataFormat α] (loc : SourceLoc) (name : α) (expected : Nat) (args : Array Tree) : ElabM Unit := do
   if p : expected < args.size then
-    logErrorMF args[expected].info.stx mf!"Unexpected argument to {name}."
+    logErrorMF args[expected].info.loc mf!"Unexpected argument to {name}."
   else if expected > args.size then
-    logErrorMF stx mf!"{name} expects {expected} arguments."
+    logErrorMF loc mf!"{name} expects {expected} arguments."
 
 /--
 This resolves a type identifer using the name of the type (as `name`) and the
 arguments (as `args`) passed into it.
 -/
 def translateTypeIdent (elabInfo : ElabInfo) (qualIdentInfo : Tree) (args : Array Tree) : ElabM Tree := do
-  let stx := qualIdentInfo.info.stx
+  let loc := qualIdentInfo.info.loc
   let tctx := qualIdentInfo.info.inputCtx
   let tpId := translateQualifiedIdent qualIdentInfo
 
   if let .name name := tpId then
     if let some binding := tctx.lookupVar name then
-      return ← resolveTypeBinding tctx stx name binding args
+      return ← resolveTypeBinding tctx loc name binding args
 
-  let some (ident, decl) ← resolveTypeOrCat stx tpId
+  let some (ident, decl) ← resolveTypeOrCat loc tpId
     | return default
 
   match decl with
   | .type decl =>
-    checkArgSize stx ident decl.argNames.size args
+    checkArgSize loc ident decl.argNames.size args
     let tpArgs ← args.mapM fun a => return (← asTypeInfo a).typeExpr
-    let tp := .ident ident tpArgs
+    let tp := .ident loc ident tpArgs
     let info : TypeInfo := { toElabInfo := elabInfo, typeExpr := tp, isInferred := false }
     return .node (.ofTypeInfo info) args
   | .syncat decl =>
-    let (_, success) ← runChecked <| checkArgSize stx ident decl.argNames.size args
+    let (_, success) ← runChecked <| checkArgSize loc ident decl.argNames.size args
     if !success then
       return default
     let mut sc : SyntaxCat := .atom ident
@@ -222,7 +240,7 @@ def translateTypeIdent (elabInfo : ElabInfo) (qualIdentInfo : Tree) (args : Arra
       | .ofCatInfo info =>
         sc := .app sc info.cat
       | _ =>
-        logError a.info.stx "Expected category."
+        logError a.info.loc "Expected category."
         return default
     let info : CatInfo := { toElabInfo := elabInfo, cat := sc }
     return .node (.ofCatInfo info) args
@@ -238,16 +256,16 @@ the root is in a normal for,.
 
 N.B. This expects that macros have already been expanded in e.
 -/
-partial def grnf (gctx : GlobalContext) (e : TypeExpr) : TypeExpr :=
+partial def headExpandTypeAlias (gctx : GlobalContext) (e : TypeExpr) : TypeExpr :=
   match e with
-  | .arrow _ _ | .ident _ _ | .bvar _ => e
-  | .fvar idx args =>
+  | .arrow .. | .ident .. | .bvar .. => e
+  | .fvar _ idx args =>
     match gctx.kindOf! idx with
     | .expr _ => panic! "Type free variable bound to expression."
     | .type params (some d) =>
       assert! params.length = args.size
       assert! !d.hasUnboundVar (bindingCount := args.size)
-      grnf gctx (d.instType args)
+      headExpandTypeAlias gctx (d.instType args)
     | .type _ none => e
 
 /--
@@ -256,8 +274,8 @@ the root is in a normal form.
 -/
 partial def rnf (tctx : TypingContext) (e : TypeExpr) : TypeExpr :=
   match e with
-  | .arrow _ _ | .ident _ _ => e
-  | .fvar idx args =>
+  | .arrow .. | .ident .. => e
+  | .fvar _ idx args =>
     let gctx := tctx.globalContext
     match gctx.kindOf! idx with
     | .expr _ => panic! "Type free variable bound to expression."
@@ -266,7 +284,7 @@ partial def rnf (tctx : TypingContext) (e : TypeExpr) : TypeExpr :=
       assert! !d.hasUnboundVar (bindingCount := args.size)
       rnf (.empty gctx) (d.instType args)
     | .type _ none => e
-  | .bvar idx =>
+  | .bvar _ idx =>
     match tctx.bindings[tctx.bindings.size - 1 - idx]!.kind with
     | .type params (some d) =>
       assert! params.isEmpty
@@ -286,7 +304,7 @@ partial def checkExpressionType (tctx : TypingContext) (itype rtype : TypeExpr) 
   let itype := rnf tctx itype
   let rtype := rnf tctx rtype
   match itype, rtype with
-  | .ident iq ia, .ident rq ra =>
+  | .ident _ iq ia, .ident _ rq ra =>
     if p : iq = rq ∧ ia.size = ra.size then do
       for i in Fin.range ia.size do
         if !(← checkExpressionType tctx ia[i] ra[i]) then
@@ -294,9 +312,9 @@ partial def checkExpressionType (tctx : TypingContext) (itype rtype : TypeExpr) 
       return true
     else
       return false
-  | .bvar ii, .bvar ri =>
+  | .bvar _ ii, .bvar _ ri =>
     return ii = ri
-  | .fvar ii ia, .fvar ri ra =>
+  | .fvar _ ii ia, .fvar _ ri ra =>
     if p : ii = ri ∧ ia.size = ra.size then do
       for i in Fin.range ia.size do
         if !(← checkExpressionType tctx ia[i] ra[i]) then
@@ -304,7 +322,7 @@ partial def checkExpressionType (tctx : TypingContext) (itype rtype : TypeExpr) 
       return true
     else
       return false
-  | .arrow ia ir, .arrow ra rr =>
+  | .arrow _ ia ir, .arrow _ ra rr =>
     return (← checkExpressionType tctx ia ra)
         && (← checkExpressionType tctx ir rr)
   | _, _ =>
@@ -355,32 +373,33 @@ partial def unifyTypes
     : ElabM (Vector (Option Tree) b.size) :=
   let ⟨argLevel, argLevelP⟩ := argLevel0
   -- Expand defined free vars at root to get head norm form
-  let expectedType := grnf tctx.globalContext expectedType
+  let expectedType := headExpandTypeAlias tctx.globalContext expectedType
+  let exprLoc := mkSourceLoc exprSyntax
   match expectedType with
-  | .ident eid ea => do
+  | .ident _ eid ea => do
     let ih := rnf tctx inferredType
     match ih with
-    | .ident iid ia =>
+    | .ident _ iid ia =>
       if eid != iid then
-        logErrorMF exprSyntax mf!"Encountered {ih} expression when {expectedType} expected."
+        logErrorMF exprLoc mf!"Encountered {ih} expression when {expectedType} expected."
         return args
       assert! ea.size = ia.size
       unifyTypeVectors b argLevel0 ea tctx exprSyntax ia args
     | _ =>
-      logErrorMF exprSyntax mf!"Encountered {ih} expression when {expectedType} expected."
+      logErrorMF exprLoc mf!"Encountered {ih} expression when {expectedType} expected."
       return args
-  | .fvar eid ea =>
+  | .fvar _ eid ea =>
     match rnf tctx inferredType with
-    | .fvar iid ia => do
+    | .fvar _ iid ia => do
       if eid != iid then
-        logErrorMF exprSyntax mf!"Encountered {inferredType} expression when {expectedType} expected."
+        logErrorMF exprLoc mf!"Encountered {inferredType} expression when {expectedType} expected."
         return args
       assert! ea.size = ia.size
       unifyTypeVectors b argLevel0 ea tctx exprSyntax ia args
     | ih => do
-      logErrorMF exprSyntax mf!"Encountered {ih} expression when {expectedType} expected."
+      logErrorMF exprLoc mf!"Encountered {ih} expression when {expectedType} expected."
       return args
-  | .bvar idx => do
+  | .bvar _ idx => do
     let .isTrue idxP := inferInstanceAs (Decidable (idx < argLevel))
       | return panic! "Invalid index"
     let typeLevel := argLevel - (idx + 1)
@@ -390,21 +409,25 @@ partial def unifyTypes
 
     match args[typeLevel] with
     | none => do
-      let einfo : ElabInfo := { stx := exprSyntax, inputCtx := tctx }
-      let info : TypeInfo := { toElabInfo := einfo, typeExpr := inferredType, isInferred := true }
+      let info : TypeInfo := {
+        loc := exprLoc
+        inputCtx := tctx
+        typeExpr := inferredType
+        isInferred := true
+      }
       return args.set typeLevel (some (.node (.ofTypeInfo info) #[]))
     | some t => do
       let .ofTypeInfo info := t.info
         | panic! "Expected type info"
       if !(← checkExpressionType tctx inferredType info.typeExpr) then
-        logErrorMF exprSyntax mf!"Expression has type {withBindings tctx.bindings (mformat inferredType)} when {withBindings tctx.bindings (mformat info.typeExpr)} expected."
+        logErrorMF exprLoc mf!"Expression has type {withBindings tctx.bindings (mformat inferredType)} when {withBindings tctx.bindings (mformat info.typeExpr)} expected."
       pure args
-  | .arrow ea er =>
+  | .arrow _ ea er =>
     match inferredType with
-    | .ident .. | .bvar _ | .fvar .. => do
-      logErrorMF exprSyntax mf!"Expected {expectedType} when {inferredType} found"
+    | .ident .. | .bvar .. | .fvar .. => do
+      logErrorMF exprLoc mf!"Expected {expectedType} when {inferredType} found"
       pure args
-    | .arrow ia ir => do
+    | .arrow _ ia ir => do
       let res ← unifyTypes b argLevel0 ea tctx exprSyntax ia args
       unifyTypes b argLevel0 er tctx exprSyntax ir res
 
@@ -420,7 +443,7 @@ private def elabManyElement (f : TypingContext → Syntax → ElabM Tree)
   pure (args.push t, rtctx)
 
 def elabOption (f : ElabArgFn) : ElabArgFn := fun tctx stx =>
-  let info : OptionInfo := { stx := stx, inputCtx := tctx }
+  let info : OptionInfo := { loc := mkSourceLoc stx, inputCtx := tctx }
   if stx.matchesNull 0 then
     pure <| .node (.ofOptionInfo info) #[]
   else do
@@ -439,18 +462,18 @@ resulting context of `tree` after the initial number of bindings given by
 `initialScope`.
 -/
 def collectNewBindingsM [Monad m] (initialScope : Nat) (tree : Tree)
-    (f : Syntax → Binding → m α) : m (Array α) := do
+    (f : SourceLoc → Binding → m α) : m (Array α) := do
   assert! (initialScope ≤ tree.info.inputCtx.bindings.size)
-  let stx := tree.info.stx
+  let loc := tree.info.loc
   let bindings := tree.resultContext.bindings.toArray
   let init : Array α := .mkEmpty (bindings.size - initialScope)
-  bindings.foldlM (init := init) (start := initialScope) fun r b => r.push <$> f stx b
+  bindings.foldlM (init := init) (start := initialScope) fun r b => r.push <$> f loc b
 
 def elabArgIndex {α} {n}
     (initialScope : Nat)
     (trees : Vector Tree n)
     (argsIndex : Option (DebruijnIndex n))
-    (f : Syntax → Binding → ElabM α) :
+    (f : SourceLoc → Binding → ElabM α) :
     ElabM (Array α) := do
   match argsIndex with
   | none => pure #[]
@@ -533,8 +556,8 @@ theorem flattenTypeApp_size (arg : Tree) (args : Array Tree) :
           omega
   termination_by sizeOf arg
 
-def logInternalError [ElabClass m] (stx : Syntax) (msg : String) : m Unit :=
-  logError stx msg
+def logInternalError {m} [ElabClass m] (loc : SourceLoc) (msg : String) : m Unit :=
+  logError loc msg
 
 /--
 Evaluate the tree as a type expression.
@@ -548,24 +571,24 @@ partial def translateSyntaxCat (tree : Tree) : ElabM SyntaxCat := do
   match op, argChildren with
   | q`Init.TypeIdent, #[ident] => do
     let tpId := translateQualifiedIdent ident
-    let some (qname, decl) ← resolveTypeOrCat ident.info.stx tpId
+    let some (qname, decl) ← resolveTypeOrCat ident.info.loc tpId
       | return default
     match decl with
     | .syncat decl =>
-      checkArgSize argInfo.stx qname decl.argNames.size args
+      checkArgSize argInfo.loc qname decl.argNames.size args
       let r : SyntaxCat := .atom qname
       args.attach.foldlM (init := r) fun r ⟨a, _⟩ => do
         have p : sizeOf a < sizeOf args := by decreasing_tactic
         return .app r (← translateSyntaxCat a)
     | _ =>
-      logError ident.info.stx s!"Expected category"; pure default
+      logError ident.info.loc s!"Expected category"; pure default
 
   | q`StrataDDL.TypeFn, _ => do
-    logError argInfo.stx s!"Expected category"
+    logError argInfo.loc s!"Expected category"
     return default
 
   | _, _ =>
-    logInternalError argInfo.stx s!"translateSyntaxCat given invalid op {op}"
+    logInternalError argInfo.loc s!"translateSyntaxCat given invalid op {op}"
     return default
 
 /--
@@ -584,27 +607,28 @@ def translateTypeExpr (tree : Tree) : ElabM TypeExpr := do
     have q := Array.sizeOf_min argChildren
     simp [feq] at p
     omega
-  let op :=
+  let opInfo :=
         match argInfo with
-        | .ofOperationInfo info => info.op.name
+        | .ofOperationInfo info => info
         | _ => panic! s!"translateBindingTypeExpr expected operator, type or cat {repr argInfo}"
+  let op := opInfo.op.name
   match op with
   | q`Init.TypeIdent => do
     let isTrue p := inferInstanceAs (Decidable (argChildren.size = 1))
       | return panic! "Invalid arguments to Init.TypeIdent"
     let ident := argChildren[0]
     let tpId := translateQualifiedIdent ident
-    let some (qname, decl) ← resolveTypeOrCat ident.info.stx tpId
+    let some (qname, decl) ← resolveTypeOrCat ident.info.loc tpId
       | return default
     match decl with
     | .type decl =>
-      checkArgSize argInfo.stx qname decl.argNames.size args
+      checkArgSize opInfo.loc qname decl.argNames.size args
       let args ← args.attach.mapM fun ⟨a, _⟩ =>
         have p : sizeOf a < sizeOf args := by decreasing_tactic
         translateTypeExpr a
-      return .ident qname args
+      return .ident opInfo.loc qname args
     | _ =>
-      logError ident.info.stx s!"Expected type"; pure default
+      logError ident.info.loc s!"Expected type"; pure default
   | q`Init.TypeArrow => do
     let isTrue p := inferInstanceAs (Decidable (argChildren.size = 2))
       | return panic! "Invalid arguments to Init.TypeArrow"
@@ -612,12 +636,12 @@ def translateTypeExpr (tree : Tree) : ElabM TypeExpr := do
     let rTree := argChildren[1]
     let aType ← translateTypeExpr aTree
     let rType ← translateTypeExpr rTree
-    return .arrow aType rType
+    return .arrow opInfo.loc aType rType
   | q`StrataDDL.TypeFn =>
-    logError argInfo.stx s!"Macros not supported"
+    logError opInfo.loc s!"Macros not supported"
     return default
   | nm =>
-    logInternalError argInfo.stx s!"translateTypeExpr given unknown constructor {nm}"
+    logInternalError opInfo.loc s!"translateTypeExpr given unknown constructor {nm}"
     return default
   termination_by tree
   decreasing_by
@@ -632,23 +656,23 @@ Evaluate the tree as a type expression.
 -/
 partial def translateBindingKind (tree : Tree) : ElabM BindingKind := do
   let (⟨argInfo, argChildren⟩, args) := flattenTypeApp tree #[]
-  let op :=
+  let opInfo :=
         match argInfo with
-        | .ofOperationInfo info => info.op.name
+        | .ofOperationInfo info => info
         | _ => panic! s!"translateBindingTypeExpr expected operator, type or cat {repr argInfo}"
-  match op, argChildren with
+  match opInfo.op.name, argChildren with
   | q`Init.TypeIdent, #[ident] => do
     let tpId := translateQualifiedIdent ident
-    let stx := ident.info.stx
-    let some (qname, decl) ← resolveTypeOrCat stx tpId
+    let loc := ident.info.loc
+    let some (qname, decl) ← resolveTypeOrCat loc tpId
       | return default
     match decl with
     | .type decl =>
-      checkArgSize argInfo.stx qname decl.argNames.size args
+      checkArgSize argInfo.loc qname decl.argNames.size args
       let args ← args.mapM translateTypeExpr
-      return .expr (.ident qname args)
+      return .expr (.ident loc qname args)
     | .syncat decl =>
-      checkArgSize argInfo.stx qname decl.argNames.size args
+      checkArgSize argInfo.loc qname decl.argNames.size args
       let r : SyntaxCat := .atom qname
       let r ← args.foldlM (init := r) fun r a => do
         return .app r (← translateSyntaxCat a)
@@ -656,12 +680,12 @@ partial def translateBindingKind (tree : Tree) : ElabM BindingKind := do
   | q`Init.TypeArrow, #[aTree, rTree] => do
     let aType ← translateTypeExpr aTree
     let rType ← translateTypeExpr rTree
-    pure <| .expr <| .arrow aType rType
+    pure <| .expr <| .arrow opInfo.loc aType rType
   | q`StrataDDL.TypeFn, _ => do
-    logError argInfo.stx s!"Macros not supported"
+    logError argInfo.loc s!"Macros not supported"
     pure default
   | _, _ =>
-    logInternalError argInfo.stx s!"translateArgDeclKind given invalid kind {op}"
+    logInternalError argInfo.loc s!"translateArgDeclKind given invalid kind {opInfo.op.name}"
     return default
 
 /--
@@ -669,6 +693,7 @@ Construct a binding from a binding spec and the arguments to a operation.
 -/
 def evalBindingSpec
     {bindings}
+    (loc : SourceLoc)
     (initSize : Nat)
     (b : BindingSpec bindings)
     (args : Vector Tree bindings.size)
@@ -676,12 +701,12 @@ def evalBindingSpec
   match b with
   | .value b =>
     let ident := evalBindingNameIndex args b.nameIndex
-    let (bindings, success) ← runChecked <| elabArgIndex initSize args b.argsIndex fun stx b =>
+    let (bindings, success) ← runChecked <| elabArgIndex initSize args b.argsIndex fun loc b =>
           match b.kind with
           | .expr tp =>
             return (b.ident, tp)
           | .type _ _ | .cat _ => do
-            logError stx "Expecting expressions in variable binding"
+            logError loc "Expecting expressions in variable binding"
             pure default
     if !success then
       return default
@@ -689,7 +714,7 @@ def evalBindingSpec
     let kind ←
           match typeTree.info with
           | .ofTypeInfo info =>
-            pure <| .expr (.mkFunType bindings info.typeExpr)
+            pure <| .expr (.mkFunType loc bindings info.typeExpr)
           | .ofCatInfo info =>
             if !b.allowCat then
               panic! s!"Cannot bind {ident} unexpected category {repr info.cat}"
@@ -707,12 +732,12 @@ def evalBindingSpec
     pure { ident, kind }
   | .type b =>
     let ident := evalBindingNameIndex args b.nameIndex
-    let params ← elabArgIndex initSize args b.argsIndex fun stx b => do
+    let params ← elabArgIndex initSize args b.argsIndex fun loc b => do
           match b.kind with
           | .type [] _ =>
             pure ()
           | .type _ _ | .expr _ | .cat _ => do
-            logError stx s!"{b.ident} must be have type Type instead of {repr b.kind}."
+            logError loc s!"{b.ident} must be have type Type instead of {repr b.kind}."
           return b.ident
     let value : Option TypeExpr :=
           match b.defIndex with
@@ -737,7 +762,7 @@ def applyNArgs (tctx : TypingContext) (e : TypeExpr) (n : Nat) := aux #[] e
   where aux (args : Array TypeExpr) (e : TypeExpr) : Except (Array TypeExpr × TypeExpr) (Vector TypeExpr n × TypeExpr) :=
     if argsLt : args.size < n then
       match rnf tctx e with
-      | .arrow a r => aux (args.push a) r
+      | .arrow _ a r => aux (args.push a) r
       | e => .error (args, e)
     else
       if argsGt : args.size > n then
@@ -755,7 +780,11 @@ def resultType! (tctx : TypingContext) (e : TypeExpr) (n : Nat) : TypeExpr :=
   | .ok (_, r) => r
   | .error (n, _) => panic! s!"{n.size} unexpected arguments to function."
 
+/--
+Returns the type of `e` in typing context `tctx`.
+-/
 partial def inferType (tctx : TypingContext) (e : Expr) : ElabM TypeExpr := do
+  -- Compute head normal form of e.
   let ⟨f, a⟩ := e.hnf
   match f with
   | .bvar idx => do
@@ -785,7 +814,7 @@ partial def inferType (tctx : TypingContext) (e : Expr) : ElabM TypeExpr := do
       some a.val[fnArgCount - i - 1]!
     let .ok tp := mtp
         | return panic! "Unexpected expandMacros failure."
-    let tp := Id.run <| tp.instTypeM fun i =>
+    let tp := Id.run <| tp.instTypeM fun _ i =>
         assert! i < fnArgCount
         let lvl := fnArgCount - i - 1
         match a.val[lvl]! with
@@ -812,15 +841,15 @@ partial def translateTypeTree (arg : Tree) : ElabM Tree := do
     | q`Init.TypeArrow, #[aTree, rTree] => do
       let aType ← translateTypeTree aTree
       let .ofTypeInfo aInfo := aType.info
-        | logError aType.info.stx s!"Expected type"; return default
+        | logError aType.info.loc s!"Expected type"; return default
       let rType ← translateTypeTree rTree
       let .ofTypeInfo rInfo := rType.info
-        | logError rType.info.stx s!"Expected type"; return default
-      let tp := .arrow aInfo.typeExpr rInfo.typeExpr
+        | logError rType.info.loc s!"Expected type"; return default
+      let tp := .arrow info.loc aInfo.typeExpr rInfo.typeExpr
       let info : TypeInfo := { toElabInfo := info.toElabInfo, typeExpr := tp, isInferred := false }
       return .node (.ofTypeInfo info) #[aType, rType]
     | _, _ =>
-      logInternalError arg.info.stx s!"translateTypeTree given invalid operation {repr op}"
+      logInternalError arg.info.loc s!"translateTypeTree given invalid operation {repr op}"
       return default
   | _ =>
     panic! s!"translateTypeExpr expected operator {repr arg}"
@@ -828,8 +857,9 @@ partial def translateTypeTree (arg : Tree) : ElabM Tree := do
 mutual
 
 partial def elabOperation (tctx : TypingContext) (stx : Syntax) : ElabM Tree := do
+  let loc := mkSourceLoc stx
   if stx.getKind = `choice then
-    logError stx s!"Parsing ambiguity {stx}"
+    logError loc s!"Parsing ambiguity {stx}"
     return default
   let some i := qualIdentKind stx
     | return panic! s!"Unknown command {stx.getKind}"
@@ -843,11 +873,10 @@ partial def elabOperation (tctx : TypingContext) (stx : Syntax) : ElabM Tree := 
   let ((args, newCtx), success) ← runChecked <| runSyntaxElaborator se decl.argDecls tctx stx.getArgs
   if !success then
     return default
-  let newBindings := decl.newBindings
-  let resultCtx ← newBindings.foldlM (init := newCtx) <| fun ctx spec => do
-    ctx.push <$> evalBindingSpec initSize spec args
-  let op : Operation := { name := i, args := args.toArray.map (·.arg) }
-  let info : OperationInfo := { stx := stx, inputCtx := tctx, op, resultCtx }
+  let resultCtx ← decl.newBindings.foldlM (init := newCtx) <| fun ctx spec => do
+    ctx.push <$> evalBindingSpec loc initSize spec args
+  let op : Operation := { ann := loc, name := i, args := args.toArray.map (·.arg) }
+  let info : OperationInfo := { loc := loc, inputCtx := tctx, op, resultCtx }
   return .node (.ofOperationInfo info) args.toArray
 
 partial def runSyntaxElaborator
@@ -885,7 +914,7 @@ partial def runSyntaxElaborator
             Tree.arg <$> trees[argLevel - i - 1]!
         match expandMacros dialects expectedType resolveArg with
         | .error () =>
-          logError astx s!"Could not infer type."
+          logError (mkSourceLoc astx) s!"Could not infer type."
         | .ok expectedType => do
           trees ← unifyTypes b ⟨argLevel, argLevelP⟩ expectedType tctx astx inferredType trees
           assert! trees[argLevel].isNone
@@ -918,7 +947,7 @@ partial def elabType (tctx : TypingContext) (stx : Syntax) : ElabM Tree := do
   | .ofTypeInfo _ =>
     pure ()
   | _ =>
-    logErrorMF stx mf!"Expected a type."
+    logErrorMF (mkSourceLoc stx) mf!"Expected a type."
   pure tree
 
 partial def catElaborator (c : SyntaxCat) : TypingContext → Syntax → ElabM Tree :=
@@ -927,13 +956,13 @@ partial def catElaborator (c : SyntaxCat) : TypingContext → Syntax → ElabM T
     elabExpr
   | .atom q`Init.Ident =>
     fun tctx stx =>
-      let info : IdentInfo := { inputCtx := tctx, stx := stx, val := stx.getId.toString }
+      let info : IdentInfo := { inputCtx := tctx, loc := mkSourceLoc stx, val := stx.getId.toString }
       pure <| .node (.ofIdentInfo info) #[]
   | .atom q`Init.Num =>
     fun tctx stx =>
       match stx.isNatLit? with
       | some v =>
-        let info : NumInfo := { inputCtx := tctx, stx := stx, val := v }
+        let info : NumInfo := { inputCtx := tctx, loc := mkSourceLoc stx, val := v }
         pure <| .node (.ofNumInfo info) #[]
       | none =>
         panic! s!"Invalid Init.Num {repr stx}"
@@ -942,7 +971,7 @@ partial def catElaborator (c : SyntaxCat) : TypingContext → Syntax → ElabM T
       match stx.isScientificLit? with
       | some (m, eIsNeg, e) =>
         let d : Decimal := { mantissa := m, exponent := if eIsNeg then .negOfNat e else .ofNat e }
-        let info : DecimalInfo := { inputCtx := tctx, stx := stx, val := d }
+        let info : DecimalInfo := { inputCtx := tctx, loc := mkSourceLoc stx, val := d }
         pure <| .node (.ofDecimalInfo info) #[]
       | none =>
         panic! s!"Invalid Init.Num {repr stx}"
@@ -950,7 +979,7 @@ partial def catElaborator (c : SyntaxCat) : TypingContext → Syntax → ElabM T
     fun tctx stx =>
       match stx.isStrLit? with
       | some s =>
-        let info : StrlitInfo := { inputCtx := tctx, stx := stx, val := s }
+        let info : StrlitInfo := { inputCtx := tctx, loc := mkSourceLoc stx, val := s }
         pure <| .node (.ofStrlitInfo info) #[]
       | none =>
         panic! s!"String not supported {stx} {stx.isStrLit?}"
@@ -969,7 +998,7 @@ partial def catElaborator (c : SyntaxCat) : TypingContext → Syntax → ElabM T
               | .ofCatInfo info => info.cat = .atom q`Init.Type
               | _ => false
         if !ok then
-          logErrorMF stx mf!"Expected a type or Type instead of {c}"
+          logErrorMF (mkSourceLoc stx) mf!"Expected a type or Type instead of {c}"
         pure tree
   | .app (.atom q`Init.Option) a =>
     elabOption (catElaborator a)
@@ -977,13 +1006,13 @@ partial def catElaborator (c : SyntaxCat) : TypingContext → Syntax → ElabM T
     let f := elabManyElement (catElaborator a)
     fun tctx stx => do
       let (args, resultCtx) ← stx.getArgs.foldlM f (#[], tctx)
-      let info : SeqInfo := { inputCtx := tctx, stx := stx, args := args.map (·.arg), resultCtx }
+      let info : SeqInfo := { inputCtx := tctx, loc := mkSourceLoc stx, args := args.map (·.arg), resultCtx }
       pure <| .node (.ofSeqInfo info) args
   | .app (.atom q`Init.CommaSepBy) a =>
     let f := elabManyElement (catElaborator a)
     fun tctx stx => do
       let (args, resultCtx) ← stx.getSepArgs.foldlM f (#[], tctx)
-      let info : CommaSepInfo := { inputCtx := tctx, stx := stx, args := args.map (·.arg), resultCtx }
+      let info : CommaSepInfo := { inputCtx := tctx, loc := mkSourceLoc stx, args := args.map (·.arg), resultCtx }
       pure <| .node (.ofCommaSepInfo info) args
   | .atom _ =>
     elabOperation
@@ -997,7 +1026,7 @@ partial def elabExpr (tctx : TypingContext) (stx : Syntax) : ElabM Tree :=
   | `Init.exprIdent =>
     let name := elabIdent stx[0]
     if let some binding := tctx.lookupVar name then
-      let einfo : ElabInfo := { stx, inputCtx := tctx }
+      let einfo : ElabInfo := { loc := mkSourceLoc stx, inputCtx := tctx }
       match binding with
       | .bvar idx k => do
         match k with
@@ -1005,10 +1034,10 @@ partial def elabExpr (tctx : TypingContext) (stx : Syntax) : ElabM Tree :=
           let info : ExprInfo := { toElabInfo := einfo, expr := .bvar idx }
           return .node (.ofExprInfo info) #[]
         | .type _params _ =>
-          logErrorMF stx mf!"{name} is a type when an expression is required."
+          logErrorMF (mkSourceLoc stx) mf!"{name} is a type when an expression is required."
           return default
         | .cat c =>
-          logErrorMF stx mf!"{name} has category {c} when an expression is required."
+          logErrorMF (mkSourceLoc stx) mf!"{name} has category {c} when an expression is required."
           return default
       | .fvar idx k =>
         match k with
@@ -1016,12 +1045,13 @@ partial def elabExpr (tctx : TypingContext) (stx : Syntax) : ElabM Tree :=
           let info : ExprInfo := { toElabInfo := einfo, expr := .fvar idx }
           return .node (.ofExprInfo info) #[]
         | _ => do
-          logError stx s!"{name} is a type when expression required."
+          logError (mkSourceLoc stx) s!"{name} is a type when expression required."
           return default
     else do
-      logError stx s!"Unknown expr identifier {name}"
+      logError (mkSourceLoc stx) s!"Unknown expr identifier {name}"
       return default
   | `Init.exprApp => do
+    let fnLoc := mkSourceLoc stx[0]
     let fn := elabIdent stx[0]
     let args := stx[2].getSepArgs
     let ((fvar, bindings), success) ← runChecked <| do
@@ -1039,18 +1069,18 @@ partial def elabExpr (tctx : TypingContext) (stx : Syntax) : ElabM Tree :=
                 pure (idx, b)
               | .error (a, r) =>
                 if a.size = 0 then
-                  logError stx[0] s!"Expected function"
+                  logError fnLoc s!"Expected function"
                 else
-                  logError stx[0] s!"Expected function with {a.size} arguments."
+                  logError fnLoc s!"Expected function with {a.size} arguments."
                 return default
             | .type _ _ =>
-              logError stx[0] s!"Expression expected."
+              logError fnLoc s!"Expression expected."
               return default
           | some (.bvar idx tp) =>
-            logError stx[0] s!"Bound functions not yet supported."
+            logError fnLoc s!"Bound functions not yet supported."
             return default
           | none =>
-            logError stx[0] s!"Unknown variable {fn}"
+            logError fnLoc s!"Unknown variable {fn}"
             return default
     if !success then
       return default
@@ -1060,9 +1090,9 @@ partial def elabExpr (tctx : TypingContext) (stx : Syntax) : ElabM Tree :=
             resultScope := none
           }
     let (args, _) ← runSyntaxElaborator se bindings tctx args
-    let e : Expr := Expr.fvar fvar
+    let e : Expr := ExprF.fvar fvar
     let e := args.toArray.foldl (init := e) fun e t => .app e t.arg
-    let info : ExprInfo := { stx := stx, inputCtx := tctx, expr := e }
+    let info : ExprInfo := { loc := mkSourceLoc stx, inputCtx := tctx, expr := e }
     return .node (.ofExprInfo info) args.toArray
   | _ => do
     let some i := qualIdentKind stx
@@ -1076,8 +1106,8 @@ partial def elabExpr (tctx : TypingContext) (stx : Syntax) : ElabM Tree :=
     let ((args, _), success) ← runChecked <| runSyntaxElaborator se fn.argDecls tctx stx.getArgs
     if !success then
       return default
-    let e := args.toArray.foldl (init := Expr.fn i) fun e t => .app e t.arg
-    let info : ExprInfo := { stx := stx, inputCtx := tctx, expr := e }
+    let e := args.toArray.foldl (init := ExprF.fn i) fun e t => .app e t.arg
+    let info : ExprInfo := { loc := mkSourceLoc stx, inputCtx := tctx, expr := e }
     return .node (.ofExprInfo info) args.toArray
 
 end
@@ -1117,7 +1147,7 @@ partial def elabCommand (leanEnv : Lean.Environment) : DeclM (Option Tree) := do
           q`Init.Command
   if leanParserState.hasError then
     for (pos, stk, err) in leanParserState.allErrors do
-      logErrorMessage stk.back <| Lean.mkErrorMessage inputContext pos stk err
+      logErrorMessage <| Lean.mkErrorMessage inputContext pos stk err
     return none
   if leanParserState.stxStack.size == 0 then
     panic! "Cmmand state is empty"
